Expressions without conversion are pure

src/coq/Theory/ExpLemmas.v
@@ -683,9 +683,44 @@ Section ExpPure.
 
   Ltac intro_pure := intros (? & ? & ? & ?) (-> & -> & ->).
 
-  Lemma expr_are_pure : forall (o : option dtyp) e, pure ⟦ e at? o ⟧e3.
+  Inductive no_conv :  exp dtyp -> Prop :=
+    no_conv_Ident x : no_conv (EXP_Ident x)
+  | no_conv_Integer z : no_conv (EXP_Integer z)
+  | no_conv_Float f : no_conv (EXP_Float f)
+  | no_conv_Double f : no_conv (EXP_Double f)
+  | no_conv_Hex f : no_conv (EXP_Hex f)
+  | no_conv_Bool b : no_conv (EXP_Bool b)
+  | no_conv_Null : no_conv (EXP_Null)
+  | no_conv_Zero_initializer : no_conv (EXP_Zero_initializer)
+  | no_conv_Cstring : forall l, (forall t x, In (t, x) l -> no_conv x) -> no_conv (EXP_Cstring l)
+  | no_conv_Undef : no_conv (EXP_Undef)
+  | no_conv_Struct : forall l, (forall t x, In (t, x) l -> no_conv x) -> no_conv (EXP_Struct l)
+  | no_conv_Packed_struct : forall l, (forall t x, In (t, x) l -> no_conv x) -> no_conv (EXP_Packed_struct l)
+  | no_conv_Array : forall l, (forall t x, In (t, x) l -> no_conv x) -> no_conv (EXP_Array l)
+  | no_conv_Vector : forall l, (forall t x, In (t, x) l -> no_conv x) -> no_conv (EXP_Vector l)
+  | no_conv_IBinop: forall b T x x', no_conv x -> no_conv x' -> no_conv (OP_IBinop b T x x')
+  | no_conv_ICmp : forall b T x x', no_conv x -> no_conv x' -> no_conv (OP_ICmp b T x x')
+  | no_conv_FBinop : forall b l T x x', no_conv x -> no_conv x' -> no_conv (OP_FBinop b l T x x')
+  | no_conv_FCmp : forall f T x x', no_conv x -> no_conv x' -> no_conv (OP_FCmp f T x x')
+  | no_conv_GetElementPtr : forall T t x l, no_conv x -> (forall t' x', In (t', x') l -> no_conv x') ->
+                                       no_conv (OP_GetElementPtr T (t, x) l)
+  | no_conv_ExtractElement : forall t x t' x', no_conv x -> no_conv x' ->
+                                            no_conv (OP_ExtractElement (t, x) (t', x'))
+  | no_conv_InsertElement : forall t x t' x' t'' x'', no_conv x -> no_conv x' -> no_conv x'' ->
+                                            no_conv (OP_InsertElement (t, x) (t', x') (t'', x''))
+  | no_conv_ShuffleVector : forall t x t' x' t'' x'', no_conv x -> no_conv x' -> no_conv x'' ->
+                                            no_conv (OP_ShuffleVector (t, x) (t', x') (t'', x''))
+  | no_conv_ExtractValue : forall t x l, no_conv x -> no_conv (OP_ExtractValue (t, x) l)
+  | no_conv_InsertValue : forall t x t' x' l, no_conv x -> no_conv x' -> no_conv (OP_InsertValue (t, x) (t', x') l)
+  | no_conv_Select : forall t x t' x' t'' x'', no_conv x -> no_conv x' -> no_conv x'' ->
+                                            no_conv (OP_Select (t, x) (t', x') (t'', x''))
+  | no_conv_Freeze : forall t x, no_conv x -> no_conv (OP_Freeze (t, x)).
+
+  Lemma expr_are_pure : forall (o : option dtyp) (e : exp dtyp),
+      no_conv e ->
+        pure ⟦ e at? o ⟧e3.
   Proof with trivial_cases.
-    intros; unfold pure.
+    intros *; unfold pure.
     revert o; induction e; simpl; intros.
 
     - destruct id; cbn.
@@ -737,7 +772,8 @@ Section ExpPure.
         * intros * IN (-> & -> & ->).
           destruct a; simpl in *.
           apply has_post_weaken with (↑ (pure_P g l m)).
-          apply (H _ IN).
+          apply (H _ IN). cbn. inv H0.
+          eauto.
           intro_pure; cbn; auto.
         * intro_pure; cbn; auto. 
       + intro_pure.
@@ -755,7 +791,7 @@ Section ExpPure.
         * intros * IN (-> & -> & ->).
           destruct a; simpl in *.
           apply has_post_weaken with (↑ (pure_P g l m)).
-          apply (H _ IN).
+          apply (H _ IN). inv H0. cbn. eauto.
           intro_pure; auto.
         * intro_pure; cbn; auto.
       + intro_pure.
@@ -772,7 +808,7 @@ Section ExpPure.
         * intros * IN (-> & -> & ->).
           destruct a; simpl in *.
           apply has_post_weaken with (↑ (pure_P g l m)).
-          apply (H _ IN).
+          apply (H _ IN). inv H0. cbn; eauto.
           intro_pure; auto.
         * intro_pure; cbn; auto.
       + intro_pure.
@@ -787,7 +823,7 @@ Section ExpPure.
         * intros * IN (-> & -> & ->).
           destruct a; simpl in *.
           apply has_post_weaken with (↑ (pure_P g l m)).
-          apply (H _ IN).
+          apply (H _ IN). cbn. inv H0. eauto.
           intro_pure; auto.
         * intro_pure; cbn; auto.
       + intro_pure.
@@ -802,7 +838,7 @@ Section ExpPure.
         * intros * IN (-> & -> & ->).
           destruct a; simpl in *.
           apply has_post_weaken with (↑ (pure_P g l m)).
-          apply (H _ IN).
+          apply (H _ IN). cbn. inv H0. eauto. 
           intro_pure; auto.
         * intro_pure; cbn; auto.
       + intro_pure.
@@ -810,11 +846,13 @@ Section ExpPure.
 
     - go.
       eapply has_post_bind_strong.
-      apply (IHe1 (Some t) g l m).
+      inv H.
+      apply (IHe1 (Some t) H2 g l m).
       intros (? & ? & ? & ?) (-> & -> & ->).
       go.
       eapply has_post_bind_strong.
-      apply (IHe2 (Some t) g l m).
+      inv H.
+      apply (IHe2 (Some t) H5 g l m).
       intro_pure.
       break_match_goal.
       + go.
@@ -849,11 +887,13 @@ Section ExpPure.
 
     - go.
       eapply has_post_bind_strong.
-      apply (IHe1 (Some t) g l m).
+      inv H.
+      specialize (IHe1 (Some t) H2 g l m). apply IHe1.
       intro_pure.
       go.
       eapply has_post_bind_strong.
-      apply (IHe2 (Some t) g l m).
+      inv H.
+      apply (IHe2 (Some t) H5 g l m).
       intro_pure.
       unfold uvalue_to_dvalue_binop.
       cbn.
@@ -867,11 +907,13 @@ Section ExpPure.
 
     - go.
       eapply has_post_bind_strong.
-      apply (IHe1 (Some t) g l m).
+      inv H.
+      apply (IHe1 (Some t) H2 g l m).
       intro_pure.
       go.
       eapply has_post_bind_strong.
-      apply (IHe2 (Some t) g l m).
+      inv H.
+      apply (IHe2 (Some t) H6 g l m).
       intro_pure.
       break_match_goal.
       + go.
@@ -906,11 +948,13 @@ Section ExpPure.
 
     - go.
       eapply has_post_bind_strong.
-      apply (IHe1 (Some t) g l m).
+      inv H.
+      apply (IHe1 (Some t) H2 g l m).
       intro_pure.
       go.
       eapply has_post_bind_strong.
-      apply (IHe2 (Some t) g l m).
+      inv H.
+      apply (IHe2 (Some t) H5 g l m).
       intro_pure.
       unfold uvalue_to_dvalue_binop.
       cbn.
@@ -922,26 +966,12 @@ Section ExpPure.
       break_match_goal...
       go...
 
-    - go.
-      eapply has_post_bind_strong.
-      apply (IHe (Some t_from) g l m).
-      intro_pure.
-      unfold uvalue_to_dvalue_uop; cbn.
-      break_match_goal.
-      go...
-      break_match_hyp; try inv_sum.
-      unfold ITree.map.
-      go.
-      apply has_post_bind_strong with (↑ (pure_P g l m)).
-      + (* What's the right way to reason about eval_conv? *)
-        admit.
-      + intro_pure.
-        go...
-
+    - inv H.
     - destruct ptrval; cbn.
       rewrite translate_bind, interp_cfg3_bind.
       eapply has_post_bind_strong.
-      apply (IHe (Some d) g l m).
+      inv H0.
+      apply (IHe (Some d) H3 g l m).
       intro_pure.
       rewrite translate_bind, interp_cfg3_bind.
       rewrite translate_map_monad.
@@ -952,7 +982,7 @@ Section ExpPure.
         * intros * IN (-> & -> & ->).
           destruct a; simpl in *.
           apply has_post_weaken with (↑ (pure_P g l m)).
-          apply (H _ IN).
+          apply (H _ IN). cbn. inv H0. eauto.
           intro_pure; auto.
         * intro_pure; cbn; auto.
       + intro_pure.
@@ -1031,7 +1061,8 @@ Section ExpPure.
     - destruct vec; cbn.
       go.
       eapply has_post_bind_strong.
-      apply (IHe (Some d) g l m).
+      inv H.
+      apply (IHe (Some d) H1 g l m).
       intro_pure.
       clear IHe.
       induction idxs as [| n idxs IH].
@@ -1047,12 +1078,15 @@ Section ExpPure.
     - destruct cnd,v1,v2; cbn.
       go.
       eapply has_post_bind_strong; [apply IHe | ].
+      cbn. inv H. eauto.
       intro_pure.
       go.
       eapply has_post_bind_strong; [apply IHe0 |]. 
+      cbn. inv H. eauto.
       intro_pure.
       go.
       eapply has_post_bind_strong; [apply IHe1 |]. 
+      cbn. inv H. eauto.
       intro_pure.
       break_match_goal.
       go...
@@ -1065,7 +1099,8 @@ Section ExpPure.
     - destruct v; cbn.
       go.
       eapply has_post_bind_strong.
-      apply (IHe (Some d) g l m).
+      inv H.
+      apply (IHe (Some d) H1 g l m).
       intro_pure.
       clear IHe.
       go.
@@ -1081,6 +1116,6 @@ Section ExpPure.
       intros (? & ? & ? & ?) (-> & -> & ->).
       go...
       
-  Admitted.
+  Qed.
 
 End ExpPure.
